cedar-lean/Cedar/Validation/Types.lean
@@ -97,12 +97,12 @@ def QualifiedType.liftBoolTypes : QualifiedType → QualifiedType
   | .optional ty => .optional ty.liftBoolTypes
   | .required ty => .required ty.liftBoolTypes
 
-def CedarType.liftBoolTypesRecord :  List (Attr × QualifiedType) → List (Attr × QualifiedType)
+def CedarType.liftBoolTypesRecord : List (Attr × QualifiedType) → List (Attr × QualifiedType)
   | [] => []
   | (a, ty)::l => (a, ty.liftBoolTypes)::(CedarType.liftBoolTypesRecord l)
 
 def RecordType.liftBoolTypes (rty : RecordType) : RecordType :=
-  .mk (CedarType.liftBoolTypesRecord rty.1)
+  .mk (CedarType.liftBoolTypesRecord rty.toList)
 
 def CedarType.liftBoolTypes : CedarType → CedarType
   | .bool bty => .bool bty.lift
