cedar-lean/Cedar/Thm/SymCC/Term/Interpret/Basic.lean
@@ -62,7 +62,7 @@ theorem interpret_term_record {I : Interpretation} {r : Map Attr Term} :
   Term.record (Map.make (r.toList.map λ (a, t) => (a, t.interpret I)))
 := by
   cases r
-  simp only [Term.interpret, recordOf, List.map₃_eq_map λ (x : (Attr × Term)) => (x.fst, x.snd.interpret I)]
+  simp [Term.interpret, recordOf, List.map₃_eq_map λ (x : (Attr × Term)) => (x.fst, x.snd.interpret I)]
 
 /--
 This tactic discharges proofs in lemmas of the form `interpret_term_app_*`,
